VCVio.lean
@@ -48,3 +48,4 @@ import VCVio.ProgramLogic.Relational.Basic
 import VCVio.ProgramLogic.Unary.DijkstraMonad
 import VCVio.ProgramLogic.Unary.Examples
 import VCVio.ProgramLogic.Unary.HoareTriple
+import VCVio.ProgramLogic.Unary.WeakestPre
